theories/interop/lang_to_mlang.v
@@ -1,14 +1,12 @@
 From Coq Require Import ssreflect.
 From stdpp Require Import strings gmap.
 From melocoton.mlanguage Require Import mlanguage.
+From melocoton.interop Require Import linking.
 From melocoton.language Require Import language.
 
 Section ToMLang.
   Context {val : Type}.
   Context (Λ : language val).
-
-  Inductive split_state : Λ.(state) → Λ.(state) → unit → Prop :=
-    split_state_refl σ : split_state σ σ tt.
 
   Local Notation prog := (gmap string Λ.(func)).
   Local Notation expr_state := ((Λ.(expr) * Λ.(state)))%type.
@@ -26,7 +24,7 @@ Section ToMLang.
 
   Lemma language_mlanguage_mixin :
     MlanguageMixin (val:=val) Λ.(of_class) Λ.(to_class) Λ.(empty_ectx) Λ.(comp_ectx) Λ.(fill)
-      split_state Λ.(apply_func) head_step.
+      Λ.(apply_func) head_step.
   Proof using.
     constructor; try apply language_mixin.
     - intros p v σ H Hstep. inversion Hstep; subst. eapply val_head_step. apply H3.
@@ -37,7 +35,6 @@ Section ToMLang.
       + destruct H as (fn & e2 & Heq1 & Heq2 & HX).
         destruct (call_head_step p f vs σ e2 σ []) as [HL HR].
         eapply wrap. 1: apply HR; by eexists. intros ? ? ( <- & <- ). apply HX.
-    - intros ? ? ? []. inversion 1; inversion 1; simplify_eq. done.
     - intros p K' K_redec e1 e1_redex σ X Heq1 Heq2 Hstep. inversion Hstep; subst.
       eapply step_by_val; try done. unfold to_val. destruct (to_class e1) as [[]|]; try congruence. exfalso. easy.
     - intros p K e σ X H. inversion H; subst.
@@ -46,7 +43,16 @@ Section ToMLang.
       + right. exists v. unfold to_val in Hv. destruct (to_class e) as [[]|]; try congruence.
   Qed.
 
-  Canonical Structure embed_lang : mlanguage val (Λ.(state)) :=
+  Canonical Structure embed_lang : mlanguage val :=
     Mlanguage language_mlanguage_mixin.
+
+  Inductive embed_split_state : Λ.(state) → Λ.(state) → unit → Prop :=
+    split_state_refl σ : embed_split_state σ σ ().
+
+  Global Program Instance embed_linkable : linkable embed_lang Λ.(state) := {
+    linking.private_state := unit;
+    linking.split_state := embed_split_state;
+  }.
+  Next Obligation. intros *. inversion 1; inversion 1; by simplify_eq. Qed.
 
 End ToMLang.
