theories/interop/linking.v
@@ -2,10 +2,29 @@ From Coq Require Import ssreflect.
 From stdpp Require Import strings gmap.
 From melocoton.mlanguage Require Import mlanguage.
 
+Class linkable {val} (Λ : mlanguage val) (public_state : Type) := Linkable {
+  private_state : Type;
+  split_state : Λ.(state) → public_state → private_state → Prop;
+  split_state_inj σ σ' pubσ privσ :
+    split_state σ pubσ privσ →
+    split_state σ' pubσ privσ →
+    σ = σ';
+}.
+
+Ltac simplify_split_state :=
+  repeat match goal with
+  | H1 : split_state _ ?x ?y,
+    H2 : split_state _ ?x ?y |- _ =>
+      pose proof (split_state_inj _ _ x y H2 H1) as ->
+  end.
+
+Module Link.
 Section Linking.
   Context {val : Type}.
-  Context {public_state : Type}.
-  Context (Λ1 Λ2 : mlanguage val public_state).
+  Context (public_state : Type).
+  Context (Λ1 Λ2 : mlanguage val).
+  Context {lk1: linkable Λ1 public_state}.
+  Context {lk2: linkable Λ2 public_state}.
 
   Definition func : Type :=
     (Λ1.(func) + Λ2.(func)).
@@ -13,19 +32,19 @@ Section Linking.
   Inductive simple_expr : Type :=
   (* The linked module produces a value
      (following one of the underlying modules producing a value) *)
-  | LinkExprV (v : val)
+  | ExprV (v : val)
   (* The linked module performs a call (corresponding to an external call
      performed by one of the underlying modules). This is not necessarily an
      external call of the linked module, it can correspond to a function
      implemented in the other linked module. *)
-  | LinkExprCall (fn_name : string) (args : list val)
+  | ExprCall (fn_name : string) (args : list val)
   (* Incoming call of one of the functions implemented by the linked module. It
      will be dispatched against the corresponding underlying module. *)
-  | LinkRunFunction (fn : func) (args : list val)
+  | RunFunction (fn : func) (args : list val)
   (* Execution of code belonging to the first underlying module. *)
-  | LinkExpr1 (e : Λ1.(mlanguage.expr))
+  | Expr1 (e : Λ1.(mlanguage.expr))
   (* Execution of code belonging to the second underlying module. *)
-  | LinkExpr2 (e : Λ2.(mlanguage.expr)).
+  | Expr2 (e : Λ2.(mlanguage.expr)).
 
   Definition ectx : Type :=
     list (Λ1.(ectx) + Λ2.(ectx)).
@@ -36,30 +55,30 @@ Section Linking.
     LkE (se: simple_expr) (k: ectx).
 
   Definition private_state : Type :=
-    (Λ1.(private_state) * Λ2.(private_state)).
+    (lk1.(private_state) * lk2.(private_state)).
   Notation LkSE se := (LkE se []).
 
   Inductive state : Type :=
-    | LinkSt (pubσ : public_state)
-             (privσ1 : Λ1.(mlanguage.private_state))
-             (privσ2 : Λ2.(mlanguage.private_state))
-    | LinkSt1 (σ1 : Λ1.(mlanguage.state)) (privσ2 : Λ2.(mlanguage.private_state))
-    | LinkSt2 (privσ1 : Λ1.(mlanguage.private_state)) (σ2 : Λ2.(mlanguage.state)).
+    | St (pubσ : public_state)
+             (privσ1 : lk1.(linking.private_state))
+             (privσ2 : lk2.(linking.private_state))
+    | St1 (σ1 : Λ1.(mlanguage.state)) (privσ2 : lk2.(linking.private_state))
+    | St2 (privσ1 : lk1.(linking.private_state)) (σ2 : Λ2.(mlanguage.state)).
 
   Inductive split_state : state → public_state → private_state → Prop :=
     | LinkSplitSt pubσ privσ1 privσ2 :
-      split_state (LinkSt pubσ privσ1 privσ2) pubσ (privσ1, privσ2).
+      split_state (St pubσ privσ1 privσ2) pubσ (privσ1, privσ2).
 
   Definition of_class (c : mixin_expr_class val) : expr :=
     match c with
-    | ExprVal v => LkSE (LinkExprV v)
-    | ExprCall fn args => LkSE (LinkExprCall fn args)
+    | ExprVal v => LkSE (ExprV v)
+    | commons.ExprCall fn args => LkSE (ExprCall fn args)
     end.
 
   Definition to_class (e : expr) : option (mixin_expr_class val) :=
     match e with
-    | LkSE (LinkExprV v) => Some (ExprVal v)
-    | LkSE (LinkExprCall fn_name args) => Some (ExprCall fn_name args)
+    | LkSE (ExprV v) => Some (ExprVal v)
+    | LkSE (ExprCall fn_name args) => Some (commons.ExprCall fn_name args)
     | _ => None
     end.
 
@@ -73,7 +92,7 @@ Section Linking.
     LkE se (k ++ K).
 
   Definition apply_func (fn : func) (args : list val) : option expr :=
-    Some (LkSE (LinkRunFunction fn args)).
+    Some (LkSE (RunFunction fn args)).
 
   Local Notation prog := (gmap string func).
 
@@ -88,63 +107,63 @@ Section Linking.
   (* Internal step of an underlying module. *)
   | Step1S e1 σ1 privσ2 (X1 : _ → Prop) X :
     prim_step (proj1_prog p) (e1, σ1) X1 →
-    (∀ e1' σ1', X1 (e1', σ1') → X (LkSE (LinkExpr1 e1'), LinkSt1 σ1' privσ2)) →
-    head_step_mrel p (LkSE (LinkExpr1 e1), LinkSt1 σ1 privσ2) X
+    (∀ e1' σ1', X1 (e1', σ1') → X (LkSE (Expr1 e1'), St1 σ1' privσ2)) →
+    head_step_mrel p (LkSE (Expr1 e1), St1 σ1 privσ2) X
   | Step2S e2 σ2 privσ1 (X2 : _ → Prop) X :
     prim_step (proj2_prog p) (e2, σ2) X2 →
-    (∀ e2' σ2', X2 (e2', σ2') → X (LkSE (LinkExpr2 e2'), LinkSt2 privσ1 σ2')) →
-    head_step_mrel p (LkSE (LinkExpr2 e2), LinkSt2 privσ1 σ2) X
+    (∀ e2' σ2', X2 (e2', σ2') → X (LkSE (Expr2 e2'), St2 privσ1 σ2')) →
+    head_step_mrel p (LkSE (Expr2 e2), St2 privσ1 σ2) X
   (* Entering a function. Change the view of the heap in the process. *)
   | RunFunction1S σ1 pubσ privσ1 privσ2 fn1 args e1 X :
     mlanguage.apply_func fn1 args = Some e1 →
-    mlanguage.split_state σ1 pubσ privσ1 →
-    X (LkSE (LinkExpr1 e1), LinkSt1 σ1 privσ2) →
-    head_step_mrel p (LkSE (LinkRunFunction (inl fn1) args), LinkSt pubσ privσ1 privσ2) X
+    linking.split_state σ1 pubσ privσ1 →
+    X (LkSE (Expr1 e1), St1 σ1 privσ2) →
+    head_step_mrel p (LkSE (RunFunction (inl fn1) args), St pubσ privσ1 privσ2) X
   | RunFunction2S σ2 pubσ privσ1 privσ2 fn2 arg e2 X :
     mlanguage.apply_func fn2 arg = Some e2 →
-    mlanguage.split_state σ2 pubσ privσ2 →
-    X (LkSE (LinkExpr2 e2), LinkSt2 privσ1 σ2) →
-    head_step_mrel p (LkSE (LinkRunFunction (inr fn2) arg), LinkSt pubσ privσ1 privσ2) X
+    linking.split_state σ2 pubσ privσ2 →
+    X (LkSE (Expr2 e2), St2 privσ1 σ2) →
+    head_step_mrel p (LkSE (RunFunction (inr fn2) arg), St pubσ privσ1 privσ2) X
   (* Producing a value when execution is finished *)
   | Val1S e1 v σ1 pubσ privσ1 privσ2 X :
     to_val e1 = Some v →
-    mlanguage.split_state σ1 pubσ privσ1 →
-    X (LkSE (LinkExprV v), LinkSt pubσ privσ1 privσ2) →
-    head_step_mrel p (LkSE (LinkExpr1 e1), LinkSt1 σ1 privσ2) X
+    linking.split_state σ1 pubσ privσ1 →
+    X (LkSE (ExprV v), St pubσ privσ1 privσ2) →
+    head_step_mrel p (LkSE (Expr1 e1), St1 σ1 privσ2) X
   | Val2S e2 v σ2 pubσ privσ1 privσ2 X :
     to_val e2 = Some v →
-    mlanguage.split_state σ2 pubσ privσ2 →
-    X (LkSE (LinkExprV v), LinkSt pubσ privσ1 privσ2) →
-    head_step_mrel p (LkSE (LinkExpr2 e2), LinkSt2 privσ1 σ2) X
+    linking.split_state σ2 pubσ privσ2 →
+    X (LkSE (ExprV v), St pubσ privσ1 privσ2) →
+    head_step_mrel p (LkSE (Expr2 e2), St2 privσ1 σ2) X
   (* Continuing execution by returning a value to its caller *)
   | Ret1S v k1 σ1 pubσ privσ1 privσ2 X :
-    mlanguage.split_state σ1 pubσ privσ1 →
-    X (LkSE (LinkExpr1 (mlanguage.fill k1 (of_val Λ1 v))), LinkSt1 σ1 privσ2) →
-    head_step_mrel p (LkE (LinkExprV v) [inl k1], LinkSt pubσ privσ1 privσ2) X
+    linking.split_state σ1 pubσ privσ1 →
+    X (LkSE (Expr1 (mlanguage.fill k1 (of_val Λ1 v))), St1 σ1 privσ2) →
+    head_step_mrel p (LkE (ExprV v) [inl k1], St pubσ privσ1 privσ2) X
   | Ret2S v k2 σ2 pubσ privσ1 privσ2 X :
-    mlanguage.split_state σ2 pubσ privσ2 →
-    X (LkSE (LinkExpr2 (mlanguage.fill k2 (of_val Λ2 v))), LinkSt2 privσ1 σ2) →
-    head_step_mrel p (LkE (LinkExprV v) [inr k2], LinkSt pubσ privσ1 privσ2) X
+    linking.split_state σ2 pubσ privσ2 →
+    X (LkSE (Expr2 (mlanguage.fill k2 (of_val Λ2 v))), St2 privσ1 σ2) →
+    head_step_mrel p (LkE (ExprV v) [inr k2], St pubσ privσ1 privσ2) X
   (* Stuck module calls bubble up as calls at the level of the linking module.
      (They may get unstuck then, if they match a function implemented by the
      other module.) *)
   | MakeCall1S k1 e1 fn_name arg σ1 pubσ privσ1 privσ2 X :
-    mlanguage.to_class e1 = Some (ExprCall fn_name arg) →
+    mlanguage.to_class e1 = Some (commons.ExprCall fn_name arg) →
     proj1_prog p !! fn_name = None →
-    mlanguage.split_state σ1 pubσ privσ1 →
-    X (LkE (LinkExprCall fn_name arg) [inl k1], LinkSt pubσ privσ1 privσ2) →
-    head_step_mrel p (LkSE (LinkExpr1 (mlanguage.fill k1 e1)), LinkSt1 σ1 privσ2) X
+    linking.split_state σ1 pubσ privσ1 →
+    X (LkE (ExprCall fn_name arg) [inl k1], St pubσ privσ1 privσ2) →
+    head_step_mrel p (LkSE (Expr1 (mlanguage.fill k1 e1)), St1 σ1 privσ2) X
   | MakeCall2S k2 e2 fn_name arg σ2 pubσ privσ1 privσ2 X :
-    mlanguage.to_class e2 = Some (ExprCall fn_name arg) →
+    mlanguage.to_class e2 = Some (commons.ExprCall fn_name arg) →
     proj2_prog p !! fn_name = None →
-    mlanguage.split_state σ2 pubσ privσ2 →
-    X (LkE (LinkExprCall fn_name arg) [inr k2], LinkSt pubσ privσ1 privσ2) →
-    head_step_mrel p (LkSE (LinkExpr2 (mlanguage.fill k2 e2)), LinkSt2 privσ1 σ2) X
+    linking.split_state σ2 pubσ privσ2 →
+    X (LkE (ExprCall fn_name arg) [inr k2], St pubσ privσ1 privσ2) →
+    head_step_mrel p (LkSE (Expr2 (mlanguage.fill k2 e2)), St2 privσ1 σ2) X
   (* Resolve an internal call to a module function *)
   | CallS fn_name fn arg σ X :
     p !! fn_name = Some fn →
-    X (LkSE (LinkRunFunction fn arg), σ) →
-    head_step_mrel p (LkSE (LinkExprCall fn_name arg), σ) X.
+    X (LkSE (RunFunction fn arg), σ) →
+    head_step_mrel p (LkSE (ExprCall fn_name arg), σ) X.
 
   Program Definition head_step (p : prog) : umrel (expr * state) :=
     {| mrel := head_step_mrel p |}.
@@ -157,7 +176,7 @@ Section Linking.
 
   Lemma mlanguage_mixin :
     MlanguageMixin (val:=val) of_class to_class empty_ectx comp_ectx fill
-      split_state apply_func head_step.
+      apply_func head_step.
   Proof using.
     constructor.
     - intros c. destruct c; reflexivity.
@@ -169,7 +188,6 @@ Section Linking.
       + intros (fn & e2 & (? & Hfn & HX)). cbn.
         unfold apply_func in Hfn; simplify_eq. econstructor; eauto.
     - intros ? ? [? ?] ? ?. rewrite /fill /=. intros. simplify_eq/=; eauto.
-    - intros σ σ' ? [? ?]. inversion 1; simplify_eq; inversion 1; simplify_eq. done.
     - intros [e k]. rewrite /fill /empty_ectx app_nil_r //.
     - intros K1 K2 [e k]. rewrite /fill /comp_ectx app_assoc //.
     - intros K [e1 k1] [e2 k2]. cbn. inversion 1; subst.
@@ -189,15 +207,27 @@ Section Linking.
       all: try match goal with H : _ |- _ => symmetry in H; apply app_singleton in H end.
       all: naive_solver.
   Qed.
-
-  Canonical Structure link_lang : mlanguage val public_state :=
-    Mlanguage mlanguage_mixin.
-
 End Linking.
+End Link.
 
-Arguments LinkSt {_ _ _ _} _ _ _.
-Arguments LinkSt1 {_ _ _ _} _ _.
-Arguments LinkSt2 {_ _ _ _} _ _.
+Arguments Link.St {_ _ _ _ _ _} _ _ _.
+Arguments Link.St1 {_ _ _ _ _ _} _ _.
+Arguments Link.St2 {_ _ _ _ _ _} _ _.
 
-Arguments LkE {_ _ _ _} _ _.
-Notation LkSE se := (LkE se []).
+Arguments Link.LkE {_ _ _} _ _.
+Notation LkSE se := (Link.LkE se []).
+
+Canonical Structure link_lang {val public_state} Λ1 Λ2 {lk1 lk2} : mlanguage val :=
+  Mlanguage (@Link.mlanguage_mixin val public_state Λ1 Λ2 lk1 lk2).
+
+Global Program Instance link_linkable
+  {val public_state} (Λ1 Λ2 : mlanguage val)
+  (lk1 : linkable Λ1 public_state)
+  (lk2 : linkable Λ2 public_state) :
+linkable (link_lang Λ1 Λ2) public_state := {
+  linking.private_state := Link.private_state _ Λ1 Λ2;
+  linking.split_state := Link.split_state _ Λ1 Λ2;
+}.
+Next Obligation.
+  intros *. inversion 1; inversion 1; by simplify_eq.
+Qed.
