theories/interop/linking_wp.v
@@ -13,19 +13,44 @@ Inductive link_state_case :=
 
 Canonical Structure link_state_caseO := leibnizO link_state_case.
 
-Class linkG Σ := LinkG {
+Class linkGS Σ := LinkGS {
   linkG_inG :> inG Σ (excl_authR (leibnizO link_state_case));
   linkG_γ : gname;
+}.
+
+Class linkableGS
+  {val pubstate hlc} (Λ : mlanguage val)
+  `{!invGS_gen hlc Σ, !mlangGS hlc val Σ Λ, !linkable Λ pubstate}
+  (public_state_interp : pubstate → iProp Σ)
+:= LinkableGS {
+  private_state_interp : private_state → iProp Σ;
+
+  state_interp_split σ pubσ privσ :
+    split_state σ pubσ privσ →
+    state_interp σ ==∗ public_state_interp pubσ ∗ private_state_interp privσ;
+
+  state_interp_join pubσ privσ :
+    public_state_interp pubσ -∗ private_state_interp privσ ==∗
+    ∃ σ, state_interp σ ∗ ⌜split_state σ pubσ privσ⌝;
+
+  splittable_at_boundary σ :
+    at_boundary Λ -∗ state_interp σ -∗ ⌜∃ pubσ privσ, split_state σ pubσ privσ⌝;
 }.
 
 Section Linking_logic.
 Context {hlc : has_lc}.
 Context {Σ : gFunctors}.
 Context {val pubstate : Type}.
-Context (Λ1 Λ2 : mlanguage val pubstate).
-Context `{linkG Σ}.
-Context `{!mlangGS hlc val pubstate Σ Λ1 public_state_interp}.
-Context `{!mlangGS hlc val pubstate Σ Λ2 public_state_interp}.
+Context (Λ1 Λ2 : mlanguage val).
+Context `{!linkGS Σ}.
+Context `{!mlangGS hlc val Σ Λ1}.
+Context `{!mlangGS hlc val Σ Λ2}.
+Context `{!invGS_gen hlc Σ}.
+Context (public_state_interp : pubstate → iProp Σ).
+Context `{!linkable Λ1 pubstate}.
+Context `{!linkable Λ2 pubstate}.
+Context `{!linkableGS Λ1 public_state_interp}.
+Context `{!linkableGS Λ2 public_state_interp}.
 
 Implicit Types P : iProp Σ.
 Implicit Types Φ : val → iProp Σ.
@@ -34,15 +59,15 @@ Implicit Types T : string -d> list val -d> (val -d> iPropO Σ) -d> iPropO Σ.
 
 Definition link_state_interp (st : (link_lang Λ1 Λ2).(state)) : iProp Σ :=
   match st with
-  | LinkSt pubσ privσ1 privσ2 =>
+  | Link.St pubσ privσ1 privσ2 =>
       own linkG_γ (●E Boundary) ∗
       public_state_interp pubσ ∗
       private_state_interp privσ1 ∗
       private_state_interp privσ2
-  | LinkSt1 σ1 privσ2 =>
+  | Link.St1 σ1 privσ2 =>
       own linkG_γ (●E In1) ∗
       state_interp σ1 ∗ private_state_interp privσ2
-  | LinkSt2 privσ1 σ2 =>
+  | Link.St2 privσ1 σ2 =>
       own linkG_γ (●E In2) ∗
       private_state_interp privσ1 ∗ state_interp σ2
   end.
@@ -68,7 +93,7 @@ Qed.
 
 Lemma link_at_boundary st :
   link_state_interp st ∗ link_state_frag Boundary -∗
-  ⌜∃ pubσ privσ1 privσ2, st = LinkSt pubσ privσ1 privσ2⌝.
+  ⌜∃ pubσ privσ1 privσ2, st = Link.St pubσ privσ1 privσ2⌝.
 Proof using.
   iIntros "[Hst Hb]". destruct st; eauto.
   all: iDestruct "Hst" as "(Hb' & _)".
@@ -77,7 +102,7 @@ Qed.
 
 Lemma link_at_in1 st :
   link_state_interp st ∗ link_state_frag In1 -∗
-  ⌜∃ σ1 privσ2, st = LinkSt1 σ1 privσ2⌝.
+  ⌜∃ σ1 privσ2, st = Link.St1 σ1 privσ2⌝.
 Proof using.
   iIntros "[Hst Hb]". destruct st; eauto.
   all: iDestruct "Hst" as "(Hb' & ?)".
@@ -86,21 +111,22 @@ Qed.
 
 Lemma link_at_in2 st :
   link_state_interp st ∗ link_state_frag In2 -∗
-  ⌜∃ privσ1 σ2, st = LinkSt2 privσ1 σ2⌝.
+  ⌜∃ privσ1 σ2, st = Link.St2 privσ1 σ2⌝.
 Proof using.
   iIntros "[Hst Hb]". destruct st; eauto.
   all: iDestruct "Hst" as "(Hb' & ?)".
   all: by iDestruct (excl_auth_eq with "Hb Hb'") as %?.
 Qed.
 
-Program Instance link_mlangGS :
-  mlangGS hlc val pubstate Σ (link_lang Λ1 Λ2) public_state_interp
-:= {
+Program Instance link_mlangGS : mlangGS hlc val Σ (link_lang Λ1 Λ2) := {
   state_interp := link_state_interp;
+  at_boundary := link_in_state Boundary;
+}.
+
+Program Instance link_linkableGS : linkableGS (link_lang Λ1 Λ2) public_state_interp := {
   private_state_interp := (λ '(privσ1, privσ2),
     own linkG_γ (●E Boundary) ∗
     private_state_interp privσ1 ∗ private_state_interp privσ2)%I;
-  at_boundary := link_in_state Boundary;
 }.
 Next Obligation.
   simpl. iIntros (σ pubσ privσ). inversion 1; subst.
@@ -108,7 +134,7 @@ Next Obligation.
 Qed.
 Next Obligation.
   simpl. iIntros (pubσ [privσ1 privσ2]) "Hpub (? & ? & ?)".
-  iModIntro. iExists (LinkSt _ _ _). by iFrame.
+  iModIntro. iExists (Link.St _ _ _). by iFrame.
 Qed.
 Next Obligation.
   iIntros (σ) "(Hb & ? & ?) Hσ".
@@ -118,10 +144,10 @@ Qed.
 
 Lemma proj1_prog_union (pe1: mlanguage.prog Λ1) (pe2: mlanguage.prog Λ2) :
   dom pe1 ## dom pe2 →
-  proj1_prog _ _ (fmap inl pe1 ∪ fmap inr pe2) = pe1.
+  Link.proj1_prog _ _ (fmap inl pe1 ∪ fmap inr pe2) = pe1.
 Proof using.
   intros Hdisj.
-  apply map_eq. intros fname. unfold proj1_prog.
+  apply map_eq. intros fname. unfold Link.proj1_prog.
   rewrite map_omap_union.
   2: { apply map_disjoint_dom. rewrite !dom_fmap//. }
   rewrite lookup_union_l.
@@ -131,10 +157,10 @@ Qed.
 
 Lemma proj2_prog_union (pe1: mlanguage.prog Λ1) (pe2: mlanguage.prog Λ2) :
   dom pe1 ## dom pe2 →
-  proj2_prog _ _ (fmap inl pe1 ∪ fmap inr pe2) = pe2.
+  Link.proj2_prog _ _ (fmap inl pe1 ∪ fmap inr pe2) = pe2.
 Proof using.
   intros Hdisj.
-  apply map_eq. intros fname. unfold proj2_prog.
+  apply map_eq. intros fname. unfold Link.proj2_prog.
   rewrite map_omap_union.
   2: { apply map_disjoint_dom. rewrite !dom_fmap//. }
   rewrite lookup_union_r.
@@ -142,10 +168,10 @@ Proof using.
   { rewrite lookup_omap /= lookup_fmap. by destruct (pe1 !! fname). }
 Qed.
 
-Definition link_environ `{!invGS_gen hlc Σ}
-  (pe1 : @prog_environ _ _ _ _ _ Λ1 _ _)
-  (pe2 : @prog_environ _ _ _ _ _ Λ2 _ _)
-: @prog_environ _ _ _ _ _ (link_lang Λ1 Λ2) _ _ :=
+Definition link_environ
+  (pe1 : prog_environ Λ1)
+  (pe2 : prog_environ Λ2)
+: prog_environ (link_lang Λ1 Λ2) :=
 {|
   prog := fmap inl (prog pe1) ∪ fmap inr (prog pe2);
   T := λ fname vs Φ,
@@ -153,9 +179,9 @@ Definition link_environ `{!invGS_gen hlc Σ}
      (T pe1 fname vs Φ ∨ T pe2 fname vs Φ))%I;
 |}.
 
-Class can_link_prog `{!invGS_gen hlc Σ}
-  (pe1 : @prog_environ _ _ _ _ _ Λ1 _ _)
-  (pe2 : @prog_environ _ _ _ _ _ Λ2 _ _)
+Class can_link_prog
+  (pe1 : prog_environ Λ1)
+  (pe2 : prog_environ Λ2)
 := CanLinkProgs {
   can_link_disj :
     dom (prog pe1) ## dom (prog pe2);
@@ -173,30 +199,30 @@ Class can_link_prog `{!invGS_gen hlc Σ}
         λ v, Φ v ∗ at_boundary Λ1 }});
 }.
 
-Lemma wp_link_call `{!invGS_gen hlc Σ}
-  (pe1 : @prog_environ _ _ _ _ _ Λ1 _ _)
-  (pe2 : @prog_environ _ _ _ _ _ Λ2 _ _)
+Lemma wp_link_call
+  (pe1 : prog_environ Λ1)
+  (pe2 : prog_environ Λ2)
   E k fn vs (Φ : val → iProp Σ) fname
 :
   let pe := link_environ pe1 pe2 in
   prog pe !! fname = Some fn →
-  WP LkE (LinkRunFunction Λ1 Λ2 fn vs) k @ pe; E {{ Φ }} -∗
-  WP LkE (LinkExprCall Λ1 Λ2 fname vs) k @ pe; E {{ Φ }}.
+  WP Link.LkE (Link.RunFunction Λ1 Λ2 fn vs) k @ pe; E {{ Φ }} -∗
+  WP Link.LkE (Link.ExprCall Λ1 Λ2 fname vs) k @ pe; E {{ Φ }}.
 Proof using.
   iIntros (pe Hfn) "Hwp".
-  iApply (@wp_unfold _ _ _ _ _ (link_lang Λ1 Λ2)). rewrite /wp_pre.
+  iApply wp_unfold. rewrite /wp_pre.
   iIntros (σ) "Hσ". iModIntro. iRight; iRight.
   iSplitR.
-  { iPureIntro. eexists (λ _, True). eexists k, (LkE _ []). split; first done.
-    eapply CallS; eauto. }
+  { iPureIntro. eexists (λ _, True). eexists k, (Link.LkE _ []). split; first done.
+    eapply Link.CallS; eauto. }
   iIntros (X Hstep'). destruct Hstep' as (K' & [se1' k1'] & ? & Hstep'); simplify_eq.
   inversion Hstep'; simplify_eq; []. simplify_map_eq.
   iModIntro. iNext. iModIntro. iExists _, _. iSplitR; first done. iFrame.
 Qed.
 
-Lemma wp_link_run_function_1 `{!invGS_gen hlc Σ}
-  (pe1 : @prog_environ _ _ _ _ _ Λ1 _ _)
-  (pe2 : @prog_environ _ _ _ _ _ Λ2 _ _)
+Lemma wp_link_run_function_1
+  (pe1 : prog_environ Λ1)
+  (pe2 : prog_environ Λ2)
   E k2 k fn arg fname (Φ : val → iProp Σ) (Ξ : val → iProp Σ)
 :
   let pe := link_environ pe1 pe2 in
@@ -208,11 +234,11 @@ Lemma wp_link_run_function_1 `{!invGS_gen hlc Σ}
   (∀ e1, ⌜apply_func fn arg = Some e1⌝ -∗
          WP e1 @ pe1; E {{ v, Ξ v ∗ at_boundary Λ1 }} -∗
          link_state_frag In1 -∗
-         WP LkE (LinkExpr1 Λ1 Λ2 e1) (inr k2 :: k) @ pe; E {{ Φ }}) -∗
-  WP LkE (LinkRunFunction Λ1 Λ2 (inl fn) arg) (inr k2 :: k) @ pe; E {{ Φ }}.
+         WP Link.LkE (Link.Expr1 Λ1 Λ2 e1) (inr k2 :: k) @ pe; E {{ Φ }}) -∗
+  WP Link.LkE (Link.RunFunction Λ1 Λ2 (inl fn) arg) (inr k2 :: k) @ pe; E {{ Φ }}.
 Proof using.
   iIntros (pe Hcan_link Hfn) "Hb Hb1 HTΞ Hwp".
-  iApply (@wp_unfold _ _ _ _ _ (link_lang Λ1 Λ2)). rewrite /wp_pre.
+  iApply wp_unfold. rewrite /wp_pre.
   iIntros (σ) "Hσ". iDestruct (link_at_boundary with "[$Hb $Hσ]") as %(pubσ&privσ1&privσ2&->).
   iRight; iRight.
   iPoseProof (can_link_spec2 _ _ _ _ E Hfn with "HTΞ") as (? Happlyfunc) "Hwpcall".
@@ -220,8 +246,8 @@ Proof using.
   iDestruct "Hσ" as "(Hob & Hpubσ & Hprivσ1 & Hprivσ2)".
   iMod (state_interp_join with "Hpubσ Hprivσ1") as (σ1) "(Hσ1 & %Hsplit)".
   iModIntro. iSplitR.
-  { iPureIntro. exists (λ _, True). eexists _, (LkE _ []). split; [done|].
-    eapply RunFunction1S; eauto. }
+  { iPureIntro. exists (λ _, True). eexists _, (Link.LkE _ []). split; [done|].
+    eapply Link.RunFunction1S; eauto. }
   iIntros (X Hstep'). destruct Hstep' as (K' & [se2' k2'] & ? & Hstep'). simpl in *; simplify_eq.
   inversion Hstep'; simplify_eq/=; []. simplify_split_state. iModIntro. iNext.
   iMod (link_state_update _ In1 with "Hob Hb") as "(Hob & Hb)".
@@ -230,9 +256,9 @@ Proof using.
   by iApply ("Hwp" with "[] Hwpcall Hb").
 Qed.
 
-Lemma wp_link_run_function_2 `{!invGS_gen hlc Σ}
-  (pe1 : @prog_environ _ _ _ _ _ Λ1 _ _)
-  (pe2 : @prog_environ _ _ _ _ _ Λ2 _ _)
+Lemma wp_link_run_function_2
+  (pe1 : prog_environ Λ1)
+  (pe2 : prog_environ Λ2)
   E k1 k fn arg fname (Φ : val → iProp Σ) (Ξ : val → iProp Σ)
 :
   let pe := link_environ pe1 pe2 in
@@ -244,11 +270,11 @@ Lemma wp_link_run_function_2 `{!invGS_gen hlc Σ}
   (∀ e2, ⌜apply_func fn arg = Some e2⌝ -∗
          WP e2 @ pe2; E {{ v, Ξ v ∗ at_boundary Λ2 }} -∗
          link_state_frag In2 -∗
-         WP LkE (LinkExpr2 Λ1 Λ2 e2) (inl k1 :: k) @ pe; E {{ Φ }}) -∗
-  WP LkE (LinkRunFunction Λ1 Λ2 (inr fn) arg) (inl k1 :: k) @ pe; E {{ Φ }}.
+         WP Link.LkE (Link.Expr2 Λ1 Λ2 e2) (inl k1 :: k) @ pe; E {{ Φ }}) -∗
+  WP Link.LkE (Link.RunFunction Λ1 Λ2 (inr fn) arg) (inl k1 :: k) @ pe; E {{ Φ }}.
 Proof using.
   iIntros (pe Hcan_link Hfn) "Hb Hb2 HTΞ Hwp".
-  iApply (@wp_unfold _ _ _ _ _ (link_lang Λ1 Λ2)). rewrite /wp_pre.
+  iApply wp_unfold. rewrite /wp_pre.
   iIntros (σ) "Hσ". iDestruct (link_at_boundary with "[$Hb $Hσ]") as %(pubσ&privσ1&privσ2&->).
   iRight; iRight.
   iPoseProof (can_link_spec1 _ _ _ _ E Hfn with "HTΞ") as (? Happlyfunc) "Hwpcall".
@@ -256,8 +282,8 @@ Proof using.
   iDestruct "Hσ" as "(Hob & Hpubσ & Hprivσ1 & Hprivσ2)".
   iMod (state_interp_join with "Hpubσ Hprivσ2") as (σ2) "(Hσ2 & %Hsplit)".
   iModIntro. iSplitR.
-  { iPureIntro. exists (λ _, True). eexists _, (LkE _ []). split; [done|].
-    eapply RunFunction2S; eauto. }
+  { iPureIntro. exists (λ _, True). eexists _, (Link.LkE _ []). split; [done|].
+    eapply Link.RunFunction2S; eauto. }
   iIntros (X Hstep'). destruct Hstep' as (K' & [se2' k2'] & ? & Hstep'). simpl in *; simplify_eq.
   inversion Hstep'; simplify_eq/=; []. simplify_split_state. iModIntro. iNext.
   iMod (link_state_update _ In2 with "Hob Hb") as "(Hob & Hb)".
@@ -266,23 +292,23 @@ Proof using.
   by iApply ("Hwp" with "[] Hwpcall Hb").
 Qed.
 
-Lemma wp_link_retval_1 `{!invGS_gen hlc Σ}
-  (pe1 : @prog_environ _ _ _ _ _ Λ1 _ _)
-  (pe2 : @prog_environ _ _ _ _ _ Λ2 _ _)
+Lemma wp_link_retval_1
+  (pe1 : prog_environ Λ1)
+  (pe2 : prog_environ Λ2)
   E k1 v (Φ : val → iProp Σ)
 :
   let pe := link_environ pe1 pe2 in
-  (link_state_frag In1 -∗ WP LkSE (LinkExpr1 Λ1 Λ2 (fill k1 (of_val Λ1 v))) @ pe; E {{ Φ }}) -∗
-  (link_state_frag Boundary -∗ WP LkE (LinkExprV Λ1 Λ2 v) [inl k1] @ pe; E {{ Φ }}).
+  (link_state_frag In1 -∗ WP LkSE (Link.Expr1 Λ1 Λ2 (fill k1 (of_val Λ1 v))) @ pe; E {{ Φ }}) -∗
+  (link_state_frag Boundary -∗ WP Link.LkE (Link.ExprV Λ1 Λ2 v) [inl k1] @ pe; E {{ Φ }}).
 Proof using.
   iIntros (pe) "Hwp Hb".
-  iApply (@wp_unfold _ _ _ _ _ (link_lang Λ1 Λ2)). rewrite /wp_pre.
+  iApply wp_unfold. rewrite /wp_pre.
   iIntros (σ) "Hσ". iDestruct (link_at_boundary with "[$Hσ $Hb]") as %(pubσ&privσ1&privσ2&->).
   iDestruct "Hσ" as "(Hob & Hpub & Hpriv1 & Hpriv2)".
   iMod (state_interp_join with "Hpub Hpriv1") as (σ1) "[Hσ1 %Hsplit]".
   iModIntro. iRight. iRight.
   iSplitR.
-  { iPureIntro. apply head_prim_reducible. exists (λ _, True). eapply Ret1S; eauto. }
+  { iPureIntro. apply head_prim_reducible. exists (λ _, True). eapply Link.Ret1S; eauto. }
   iIntros (X Hstep'). destruct Hstep' as (K' & [se1' k1'] & ? & Hstep'). simplify_eq/=.
   inversion Hstep'; simplify_eq/=; []. simplify_split_state.
   iModIntro. iNext.
@@ -290,23 +316,23 @@ Proof using.
   iModIntro. iExists _, _. iSplitR; first done. iFrame. iApply "Hwp". iFrame.
 Qed.
 
-Lemma wp_link_retval_2 `{!invGS_gen hlc Σ}
-  (pe1 : @prog_environ _ _ _ _ _ Λ1 _ _)
-  (pe2 : @prog_environ _ _ _ _ _ Λ2 _ _)
+Lemma wp_link_retval_2
+  (pe1 : prog_environ Λ1)
+  (pe2 : prog_environ Λ2)
   E k2 v (Φ : val → iProp Σ)
 :
   let pe := link_environ pe1 pe2 in
-  (link_state_frag In2 -∗ WP LkSE (LinkExpr2 Λ1 Λ2 (fill k2 (of_val Λ2 v))) @ pe; E {{ Φ }}) -∗
-  (link_state_frag Boundary -∗ WP LkE (LinkExprV Λ1 Λ2 v) [inr k2] @ pe; E {{ Φ }}).
+  (link_state_frag In2 -∗ WP LkSE (Link.Expr2 Λ1 Λ2 (fill k2 (of_val Λ2 v))) @ pe; E {{ Φ }}) -∗
+  (link_state_frag Boundary -∗ WP Link.LkE (Link.ExprV Λ1 Λ2 v) [inr k2] @ pe; E {{ Φ }}).
 Proof using.
   iIntros (pe) "Hwp Hb".
-  iApply (@wp_unfold _ _ _ _ _ (link_lang Λ1 Λ2)). rewrite /wp_pre.
+  iApply wp_unfold. rewrite /wp_pre.
   iIntros (σ) "Hσ". iDestruct (link_at_boundary with "[$Hσ $Hb]") as %(pubσ&privσ1&privσ2&->).
   iDestruct "Hσ" as "(Hob & Hpub & Hpriv1 & Hpriv2)".
   iMod (state_interp_join with "Hpub Hpriv2") as (σ2) "[Hσ2 %Hsplit]".
   iModIntro. iRight. iRight.
   iSplitR.
-  { iPureIntro. apply head_prim_reducible. eexists (λ _, True). eapply Ret2S; eauto. }
+  { iPureIntro. apply head_prim_reducible. eexists (λ _, True). eapply Link.Ret2S; eauto. }
   iIntros (X Hstep'). destruct Hstep' as (K' & [se2' k2'] & ? & Hstep'). simplify_eq/=.
   inversion Hstep'; simplify_eq/=; []. simplify_split_state.
   iModIntro. iNext.
@@ -314,9 +340,9 @@ Proof using.
   iModIntro. iExists _, _. iSplitR; first done. iFrame. iApply "Hwp". iFrame.
 Qed.
 
-Lemma wp_link_extcall_1 `{!invGS_gen hlc Σ}
-  (pe1 : @prog_environ _ _ _ _ _ Λ1 _ _)
-  (pe2 : @prog_environ _ _ _ _ _ Λ2 _ _)
+Lemma wp_link_extcall_1
+  (pe1 : prog_environ Λ1)
+  (pe2 : prog_environ Λ2)
   E k1 fn_name arg (Φ : val → iProp Σ) (Ξ : val → iProp Σ)
 :
   let pe := link_environ pe1 pe2 in
@@ -328,14 +354,14 @@ Lemma wp_link_extcall_1 `{!invGS_gen hlc Σ}
   (▷ ∀ r, WP fill k1 (of_class Λ1 (ExprVal r)) @ pe1; E {{ λ v, Φ v ∗ at_boundary Λ1 }} -∗
         link_state_frag Boundary -∗
         at_boundary Λ2 -∗
-        WP LkE (LinkExprV Λ1 Λ2 r) [inl k1] @ pe; E {{ λ v, Φ v ∗ at_boundary (link_lang Λ1 Λ2) }}) -∗
+        WP Link.LkE (Link.ExprV Λ1 Λ2 r) [inl k1] @ pe; E {{ λ v, Φ v ∗ at_boundary (link_lang Λ1 Λ2) }}) -∗
   at_boundary (link_lang Λ1 Λ2) -∗
-  WP LkE (LinkExprCall Λ1 Λ2 fn_name arg) [inl k1] @ pe; E {{ λ v, Φ v ∗ at_boundary (link_lang Λ1 Λ2) }}.
+  WP Link.LkE (Link.ExprCall Λ1 Λ2 fn_name arg) [inl k1] @ pe; E {{ λ v, Φ v ∗ at_boundary (link_lang Λ1 Λ2) }}.
 Proof using.
   iIntros (pe Hfn1 Hfn2) "HTΞ HΞ Hwp (Hb & Hb1 & Hb2)".
   assert (Hpef: prog pe !! fn_name = None).
   { apply lookup_union_None. rewrite !lookup_fmap Hfn1 Hfn2 //. }
-  iApply (@wp_unfold _ _ _ _ _ (link_lang Λ1 Λ2)). rewrite /wp_pre.
+  iApply wp_unfold. rewrite /wp_pre.
   iIntros (σ) "Hσ". iDestruct (link_at_boundary with "[$Hσ $Hb]") as %(pubσ&privσ1&privσ2&->).
   iModIntro. iRight; iLeft. iExists _, _, [inl k1]. iSplitR; [by eauto|].
   iSplitR; first by eauto. iFrame "Hσ Hb Hb1 Hb2". iExists Ξ. iSplitL "HTΞ".
@@ -346,9 +372,9 @@ Proof using.
   iApply ("Hwp" with "HΞ Hb Hb2").
 Qed.
 
-Lemma wp_link_extcall_2 `{!invGS_gen hlc Σ}
-  (pe1 : @prog_environ _ _ _ _ _ Λ1 _ _)
-  (pe2 : @prog_environ _ _ _ _ _ Λ2 _ _)
+Lemma wp_link_extcall_2
+  (pe1 : prog_environ Λ1)
+  (pe2 : prog_environ Λ2)
   E k2 fn_name arg (Φ : val → iProp Σ) (Ξ : val → iProp Σ)
 :
   let pe := link_environ pe1 pe2 in
@@ -360,14 +386,14 @@ Lemma wp_link_extcall_2 `{!invGS_gen hlc Σ}
   (▷ ∀ r, WP fill k2 (of_class Λ2 (ExprVal r)) @ pe2; E {{ λ v, Φ v ∗ at_boundary Λ2 }} -∗
         link_state_frag Boundary -∗
         at_boundary Λ1 -∗
-        WP LkE (LinkExprV Λ1 Λ2 r) [inr k2] @ pe; E {{ λ v, Φ v ∗ at_boundary (link_lang Λ1 Λ2) }}) -∗
+        WP Link.LkE (Link.ExprV Λ1 Λ2 r) [inr k2] @ pe; E {{ λ v, Φ v ∗ at_boundary (link_lang Λ1 Λ2) }}) -∗
   at_boundary (link_lang Λ1 Λ2) -∗
-  WP LkE (LinkExprCall Λ1 Λ2 fn_name arg) [inr k2] @ pe; E {{ λ v, Φ v ∗ at_boundary (link_lang Λ1 Λ2) }}.
+  WP Link.LkE (Link.ExprCall Λ1 Λ2 fn_name arg) [inr k2] @ pe; E {{ λ v, Φ v ∗ at_boundary (link_lang Λ1 Λ2) }}.
 Proof using.
   iIntros (pe Hfn1 Hfn2) "HTΞ HΞ Hwp (Hb & Hb1 & Hb2)".
   assert (Hpef: prog pe !! fn_name = None).
   { apply lookup_union_None. rewrite !lookup_fmap Hfn1 Hfn2 //. }
-  iApply (@wp_unfold _ _ _ _ _ (link_lang Λ1 Λ2)). rewrite /wp_pre.
+  iApply wp_unfold. rewrite /wp_pre.
   iIntros (σ) "Hσ". iDestruct (link_at_boundary with "[$Hσ $Hb]") as %(pubσ&privσ1&privσ2&->).
   iModIntro. iRight; iLeft. iExists _, _, [inr k2]. iSplitR; [by eauto|].
   iSplitR; first by eauto. iFrame "Hσ Hb Hb1 Hb2". iExists Ξ. iSplitL "HTΞ".
@@ -378,15 +404,15 @@ Proof using.
   iApply ("Hwp" with "HΞ Hb Hb1").
 Qed.
 
-Lemma link_head_step_call_ext_1_inv `{!invGS_gen hlc Σ} pe1 pe2 K f vs σ1 privσ2 X :
+Lemma link_head_step_call_ext_1_inv pe1 pe2 K f vs σ1 privσ2 X :
   let pe := link_environ pe1 pe2 in
   can_link_prog pe1 pe2 →
   prog pe1 !! f = None →
-  head_step (prog pe) (LkSE (LinkExpr1 Λ1 Λ2 (fill K (of_class Λ1 (ExprCall f vs)))),
-                       LinkSt1 σ1 privσ2) X →
+  head_step (prog pe) (LkSE (Link.Expr1 Λ1 Λ2 (fill K (of_class Λ1 (ExprCall f vs)))),
+                       Link.St1 σ1 privσ2) X →
   ∃ pubσ privσ1 k,
     K = comp_ectx k empty_ectx ∧
-    X (LkE (LinkExprCall Λ1 Λ2 f vs) [inl k], LinkSt pubσ privσ1 privσ2) ∧
+    X (Link.LkE (Link.ExprCall Λ1 Λ2 f vs) [inl k], Link.St pubσ privσ1 privσ2) ∧
     split_state σ1 pubσ privσ1.
 Proof using.
   intros pe Hcan_link Hf Hstep. inversion Hstep; subst; simplify_eq.
@@ -396,7 +422,7 @@ Proof using.
   { exfalso. match goal with H:_|-_ => apply mk_is_Some in H; apply fill_val in H; destruct H as [? HH] end.
     rewrite /to_val to_of_class // in HH. }
   match goal with H: fill _ _ = fill _ _ |- _ => rename H into Hfill end.
-  match goal with H: proj1_prog _ _ _ !! _ = None |- _ => rename H into Hnofn end.
+  match goal with H: Link.proj1_prog _ _ _ !! _ = None |- _ => rename H into Hnofn end.
   rewrite proj1_prog_union in Hnofn;[|apply Hcan_link].
   pose proof (call_in_ctx_to_val _ _ _ _ _ Hfill) as [[K'' ->]|Hval].
   2: { exfalso. unfold to_val in Hval. destruct Hval. by repeat case_match. }
@@ -409,15 +435,15 @@ Proof using.
   rewrite fill_empty to_of_class in Hcall. by simplify_eq/=.
 Qed.
 
-Lemma link_head_step_call_ext_2_inv `{!invGS_gen hlc Σ} pe1 pe2 K f vs σ2 privσ1 X :
+Lemma link_head_step_call_ext_2_inv pe1 pe2 K f vs σ2 privσ1 X :
   let pe := link_environ pe1 pe2 in
   can_link_prog pe1 pe2 →
   prog pe2 !! f = None →
-  head_step (prog pe) (LkSE (LinkExpr2 Λ1 Λ2 (fill K (of_class Λ2 (ExprCall f vs)))),
-                       LinkSt2 privσ1 σ2) X →
+  head_step (prog pe) (LkSE (Link.Expr2 Λ1 Λ2 (fill K (of_class Λ2 (ExprCall f vs)))),
+                       Link.St2 privσ1 σ2) X →
   ∃ pubσ privσ2 k,
     K = comp_ectx k empty_ectx ∧
-    X (LkE (LinkExprCall Λ1 Λ2 f vs) [inr k], LinkSt pubσ privσ1 privσ2) ∧
+    X (Link.LkE (Link.ExprCall Λ1 Λ2 f vs) [inr k], Link.St pubσ privσ1 privσ2) ∧
     split_state σ2 pubσ privσ2.
 Proof using.
   intros pe Hcan_link Hf Hstep. inversion Hstep; subst; simplify_eq.
@@ -426,7 +452,7 @@ Proof using.
   { exfalso. match goal with H:_|-_ => apply mk_is_Some in H; apply fill_val in H; destruct H as [? HH] end.
     rewrite /to_val to_of_class // in HH. }
   match goal with H: fill _ _ = fill _ _ |- _ => rename H into Hfill end.
-  match goal with H: proj2_prog _ _ _ !! _ = None |- _ => rename H into Hnofn end.
+  match goal with H: Link.proj2_prog _ _ _ !! _ = None |- _ => rename H into Hnofn end.
   rewrite proj2_prog_union in Hnofn;[|apply Hcan_link].
   pose proof (call_in_ctx_to_val _ _ _ _ _ Hfill) as [[K'' ->]|Hval].
   2: { exfalso. unfold to_val in Hval. destruct Hval. by repeat case_match. }
@@ -439,25 +465,25 @@ Proof using.
   rewrite fill_empty to_of_class in Hcall. by simplify_eq/=.
 Qed.
 
-Lemma wp_link_run `{!invGS_gen hlc Σ}
-  (pe1 : @prog_environ _ _ _ _ _ Λ1 _ _)
-  (pe2 : @prog_environ _ _ _ _ _ Λ2 _ _)
+Lemma wp_link_run
+  (pe1 : prog_environ Λ1)
+  (pe2 : prog_environ Λ2)
   E
 :
   let pe := link_environ pe1 pe2 in
   can_link_prog pe1 pe2 →
   ⊢ □ (
     (∀ e1 Φ, WP e1 @ pe1; E {{ λ v, Φ v ∗ at_boundary Λ1 }} -∗ link_in_state In1 -∗
-             WP (LkSE (LinkExpr1 Λ1 Λ2 e1)) @ pe; E {{ λ v, Φ v ∗ link_in_state Boundary }}) ∗
+             WP (LkSE (Link.Expr1 Λ1 Λ2 e1)) @ pe; E {{ λ v, Φ v ∗ link_in_state Boundary }}) ∗
     (∀ e2 Φ, WP e2 @ pe2; E {{ λ v, Φ v ∗ at_boundary Λ2 }} -∗ link_in_state In2 -∗
-             WP (LkSE (LinkExpr2 Λ1 Λ2 e2)) @ pe; E {{ λ v, Φ v ∗ link_in_state Boundary }})
+             WP (LkSE (Link.Expr2 Λ1 Λ2 e2)) @ pe; E {{ λ v, Φ v ∗ link_in_state Boundary }})
   ).
 Proof using.
   intros pe Hcan_link. iLöb as "IH". iModIntro. iSplitL.
   (* Case 1: running Λ1 *)
   { iIntros (e1 Φ) "Hwp [Hb Hb2]".
     rewrite wp_unfold. rewrite /wp_pre.
-    iApply (@wp_unfold _ _ _ _ _ (link_lang Λ1 Λ2)). rewrite /wp_pre.
+    iApply wp_unfold. rewrite /wp_pre.
     iIntros (σ) "Hσ". iDestruct (link_at_in1 with "[$Hb $Hσ]") as %(σ1 & privσ2 & ->).
     iDestruct "Hσ" as "(Hob & Hσ1 & Hpriv2)".
     iMod ("Hwp" $! σ1 with "[$Hσ1]") as "[Hwp|[Hwp|Hwp]]".
@@ -465,30 +491,31 @@ Proof using.
     (* WP: value case *)
     { iDestruct "Hwp" as (v ->) "[Hσ [HΦ Hb1]]".
       iModIntro. iRight; iRight.
-      (* administrative step Val1S: LinkExpr1 ~> LinkExprV *)
+      (* administrative step Val1S: Link.Expr1 ~> Link.ExprV *)
       iDestruct (@splittable_at_boundary with "Hb1 Hσ") as %(pubσ&privσ1&Hsplitσ1).
-      assert (Hhred: head_reducible (prog pe) (LkSE (LinkExpr1 Λ1 Λ2 (of_class Λ1 (ExprVal v)))) (LinkSt1 σ1 privσ2)).
-      { exists (λ _, True). eapply Val1S; eauto. rewrite /to_val to_of_class //=. }
+      assert (Hhred: head_reducible (prog pe) (LkSE (Link.Expr1 Λ1 Λ2 (of_class Λ1 (ExprVal v)))) (Link.St1 σ1 privσ2)).
+      { exists (λ _, True). eapply Link.Val1S; eauto. rewrite /to_val to_of_class //=. }
       iSplitR; [iPureIntro; by apply head_prim_reducible|].
       iIntros (X Hstep). apply head_reducible_prim_step in Hstep; [|done].
       inversion Hstep; simplify_eq/=.
       { exfalso. by match goal with H:_ |- _ => apply val_prim_step in H end. }
-      { rewrite /to_val to_of_class in H3; simplify_eq/=.
-        iMod (@state_interp_split _ _ _ _ Λ1 with "Hσ") as "[Hpriv1 Hpub]"; first by eauto.
+      { match goal with H : to_val (of_class _ _) = _ |- _ => rewrite to_of_val in H; simplify_eq end.
+        iMod (state_interp_split with "Hσ") as "[Hpriv1 Hpub]"; first by eauto.
         iExists _, _. iSplitR; first done.
         iMod (link_state_update _ Boundary with "Hob Hb") as "[Hob Hb]".
         do 3 iModIntro. iFrame. by iApply wp_value. }
       { exfalso.
         assert (is_Some (to_val e1)) as [? ?].
-        { eapply fill_val. eexists. unfold to_val. erewrite H0. rewrite to_of_class//. }
-        unfold to_val in H1. repeat case_match; congruence. } }
+        { eapply fill_val. eexists. unfold to_val.
+          match goal with H : fill _ _ = _ |- _ => erewrite H end. rewrite to_of_class//. }
+        unfold to_val in *. repeat case_match; congruence. } }
 
     (* WP: call case *)
     { iDestruct "Hwp" as (f vs K -> Hf) "(Hb1 & Hσ1 & Hcall)". iModIntro. iRight; iRight.
-      (* administrative step MakeCall1S: LinkExpr1 ~> LinkExprCall *)
+      (* administrative step MakeCall1S: Link.Expr1 ~> Link.ExprCall *)
       iDestruct (@splittable_at_boundary with "Hb1 Hσ1") as %(pubσ&privσ1&Hsplitσ1).
-      assert (head_reducible (prog pe) (LkSE (LinkExpr1 Λ1 Λ2 (fill K (of_class Λ1 (ExprCall f vs))))) (LinkSt1 σ1 privσ2)).
-      { exists (λ _, True). eapply MakeCall1S; eauto. by rewrite to_of_class.
+      assert (head_reducible (prog pe) (LkSE (Link.Expr1 Λ1 Λ2 (fill K (of_class Λ1 (ExprCall f vs))))) (Link.St1 σ1 privσ2)).
+      { exists (λ _, True). eapply Link.MakeCall1S; eauto. by rewrite to_of_class.
         rewrite proj1_prog_union; [done | apply Hcan_link]. }
       iSplitR; [iPureIntro; by apply head_prim_reducible|].
       iIntros (X Hstep). apply head_reducible_prim_step in Hstep;[|done].
@@ -496,7 +523,7 @@ Proof using.
       eapply link_head_step_call_ext_1_inv in Hstep as (pubσ&privσ1&k1&->&?&?); eauto.
 
       iDestruct "Hcall" as (Ξ) "[HTΞ HΞ]".
-      iMod (@state_interp_split _ _ _ _ Λ1 with "Hσ1") as "[Hpriv1 Hpub]"; first done.
+      iMod (state_interp_split with "Hσ1") as "[Hpriv1 Hpub]"; first done.
       iMod (link_state_update _ Boundary with "Hob Hb") as "[Hob Hb]".
       do 3 iModIntro. iExists _, _. iSplitR; first done. simpl.
       iFrame "Hob Hpub Hpriv1 Hpriv2".
@@ -509,21 +536,21 @@ Proof using.
         assert (prog pe !! f = Some (inr fn2)) as Hpef.
         { rewrite lookup_union_r lookup_fmap. by rewrite Hf2. by rewrite Hf. }
 
-        (* administrative step CallS: LinkExprCall ~> LinkRunFunction *)
+        (* administrative step CallS: Link.ExprCall ~> LinkRunFunction *)
         iApply wp_link_call; first done.
-        (* administrative step RunFunction2S: LinkRunFunction ~> LinkExpr2 *)
+        (* administrative step RunFunction2S: LinkRunFunction ~> Link.Expr2 *)
         iApply (wp_link_run_function_2 with "Hb Hb2 HTΞ"); first done.
         iIntros (e2 He2) "Hwpcall Hb".
 
-        progress change (LkE (LinkExpr2 Λ1 Λ2 e2) [inl k1]) with
-          (linking.fill _ _ ([inl k1]:ectx (link_lang Λ1 Λ2)) (LkSE (LinkExpr2 Λ1 Λ2 e2))).
-        iApply (@wp_bind _ _ _ _ _ (link_lang Λ1 Λ2)).
-        iApply ((@wp_wand _ _ _ _ _ (link_lang Λ1 Λ2)) with "[Hwpcall Hb Hb1]").
+        progress change (Link.LkE (Link.Expr2 Λ1 Λ2 e2) [inl k1]) with
+          (Link.fill _ _ ([inl k1]:ectx (link_lang Λ1 Λ2)) (LkSE (Link.Expr2 Λ1 Λ2 e2))).
+        iApply wp_bind.
+        iApply (wp_wand with "[Hwpcall Hb Hb1]").
         { iDestruct "IH" as "#[_ IH2]". iApply ("IH2" with "Hwpcall [$Hb $Hb1]"). }
         iIntros (r) "[Hr (Hb & Hb1 & Hb2)]". iSpecialize ("HΞ" $! r).
         rewrite -fill_comp fill_empty. simpl.
 
-        (* administrative step Ret1S: LinkExprV ~> LinkExpr1 *)
+        (* administrative step Ret1S: Link.ExprV ~> Link.Expr1 *)
         iApply (wp_link_retval_1 with "[-Hb] Hb"). iIntros "Hb".
         (* continue the execution by induction *)
         iDestruct "IH" as "#[IH1 _]". iApply ("IH1" with "[-Hb Hb2] [$Hb $Hb2]"). unfold of_val.
@@ -533,64 +560,64 @@ Proof using.
         iApply (wp_link_extcall_1 with "HTΞ HΞ [] [$Hb $Hb1 $Hb2]"); auto.
         iNext.
         iIntros (r) "HΞ Hb Hb2".
-        (* administrative step Ret1S: LinkExprV ~> LinkExpr1 *)
+        (* administrative step Ret1S: Link.ExprV ~> Link.Expr1 *)
         iApply (wp_link_retval_1 with "[-Hb] Hb"). iIntros "Hb".
         (* continue the execution by induction *)
         iDestruct "IH" as "#[IH1 _]". iApply ("IH1" with "HΞ [$Hb $Hb2]"). } }
 
     { (* WP: step case *)
       iDestruct "Hwp" as (Hred) "Hwp". iModIntro. iRight; iRight.
-      assert (head_reducible (prog pe) (LkSE (LinkExpr1 Λ1 Λ2 e1)) (LinkSt1 σ1 privσ2)).
+      assert (head_reducible (prog pe) (LkSE (Link.Expr1 Λ1 Λ2 e1)) (Link.St1 σ1 privσ2)).
       { destruct Hred as (? & Hstep). exists (λ _, True).
-        eapply Step1S. rewrite proj1_prog_union; [| apply Hcan_link]. all: eauto. }
+        eapply Link.Step1S. rewrite proj1_prog_union; [| apply Hcan_link]. all: eauto. }
       iSplitR; [by iPureIntro; apply head_prim_reducible|].
       iIntros (X Hstep). apply head_reducible_prim_step in Hstep;[|done].
       inversion Hstep; simplify_eq.
       { (* non-vacuous case: step in Λ1 *)
-        clear Hstep. rename H5 into Hstep.
+        clear Hstep. rename H4 into Hstep.
         rewrite proj1_prog_union in Hstep; [|apply Hcan_link].
         iSpecialize ("Hwp" $! _ Hstep). iMod "Hwp". iIntros "!>!>". iMod "Hwp" as (e' σ' HX) "[Hσ Hwp]".
         iModIntro. iExists _, _. iSplitR; [iPureIntro; naive_solver|]. iFrame "Hσ Hob Hpriv2".
         iDestruct "IH" as "[IH1 _]". iApply ("IH1" with "Hwp [$Hb $Hb2]"). }
       { exfalso. apply reducible_not_val in Hred. congruence. }
       { exfalso. clear Hstep. erewrite <-(of_to_class e0) in Hred; [|eassumption].
-        rewrite proj1_prog_union in H5;[|apply Hcan_link].
+        rewrite proj1_prog_union in H4;[|apply Hcan_link].
         destruct Hred as (?&Hred). eapply extcall_ctx_irreducible; eauto. } } }
 
   (* Case 2: running Λ2 *)
   { iIntros (e2 Φ) "Hwp [Hb Hb1]".
-    rewrite wp_unfold. rewrite /wp_pre.
-    iApply (@wp_unfold _ _ _ _ _ (link_lang Λ1 Λ2)). rewrite /wp_pre.
+    rewrite wp_unfold. rewrite /wp_pre. iApply wp_unfold. rewrite /wp_pre.
     iIntros (σ) "Hσ". iDestruct (link_at_in2 with "[$Hb $Hσ]") as %(privσ1 & σ2 & ->).
     iDestruct "Hσ" as "(Hob & Hpriv1 & Hσ2)".
     iMod ("Hwp" $! σ2 with "[$Hσ2]") as "[Hwp|[Hwp|Hwp]]".
 
     (* WP: value case *)
     { iDestruct "Hwp" as (v ->) "[Hσ [HΦ Hb2]]". iModIntro. iRight; iRight.
-      (* administrative step Val2S: LinkExpr2 ~> LinkExprV *)
+      (* administrative step Val2S: Link.Expr2 ~> Link.ExprV *)
       iDestruct (@splittable_at_boundary with "Hb2 Hσ") as %(pubσ&privσ2&Hsplitσ2).
-      assert (Hhred: head_reducible (prog pe) (LkSE (LinkExpr2 Λ1 Λ2 (of_class Λ2 (ExprVal v)))) (LinkSt2 privσ1 σ2)).
-      { exists (λ _, True). eapply Val2S; eauto. rewrite /to_val to_of_class //=. }
+      assert (Hhred: head_reducible (prog pe) (LkSE (Link.Expr2 Λ1 Λ2 (of_class Λ2 (ExprVal v)))) (Link.St2 privσ1 σ2)).
+      { exists (λ _, True). eapply Link.Val2S; eauto. rewrite /to_val to_of_class //=. }
       iSplitR; [iPureIntro; by apply head_prim_reducible|].
       iIntros (X Hstep). apply head_reducible_prim_step in Hstep; [|done].
       inversion Hstep; simplify_eq/=.
       { exfalso. by match goal with H:_ |- _ => apply val_prim_step in H end. }
-      { rewrite /to_val to_of_class in H3; simplify_eq/=.
-        iMod (@state_interp_split _ _ _ _ Λ2 with "Hσ") as "[Hpriv2 Hpub]"; first by eauto.
+      { match goal with H : to_val (of_class _ _) = _ |- _ => rewrite to_of_val in H; simplify_eq end.
+        iMod (state_interp_split with "Hσ") as "[Hpriv2 Hpub]"; first by eauto.
         iExists _, _. iSplitR; first done.
         iMod (link_state_update _ Boundary with "Hob Hb") as "[Hob Hb]".
         do 3 iModIntro. iFrame. by iApply wp_value. }
       { exfalso.
         assert (is_Some (to_val e2)) as [? ?].
-        { eapply fill_val. eexists. unfold to_val. erewrite H0. rewrite to_of_class//. }
-        unfold to_val in H1. repeat case_match; congruence. } }
+        { eapply fill_val. eexists. unfold to_val.
+          match goal with H : fill _ _ = _ |- _ => erewrite H end. rewrite to_of_class//. }
+        unfold to_val in *. repeat case_match; congruence. } }
 
     (* WP: call case *)
     { iDestruct "Hwp" as (f vs K -> Hf) "(Hb2 & Hσ2 & Hcall)". iModIntro. iRight; iRight.
-      (* administrative step MakeCall1S: LinkExpr2 ~> LinkExprCall *)
+      (* administrative step MakeCall1S: Link.Expr2 ~> Link.ExprCall *)
       iDestruct (@splittable_at_boundary with "Hb2 Hσ2") as %(pubσ&privσ2&Hsplitσ2).
-      assert (head_reducible (prog pe) (LkSE (LinkExpr2 Λ1 Λ2 (fill K (of_class Λ2 (ExprCall f vs))))) (LinkSt2 privσ1 σ2)).
-      { exists (λ _, True). eapply MakeCall2S; eauto. by rewrite to_of_class.
+      assert (head_reducible (prog pe) (LkSE (Link.Expr2 Λ1 Λ2 (fill K (of_class Λ2 (ExprCall f vs))))) (Link.St2 privσ1 σ2)).
+      { exists (λ _, True). eapply Link.MakeCall2S; eauto. by rewrite to_of_class.
         rewrite proj2_prog_union; [done | apply Hcan_link]. }
       iSplitR; [iPureIntro; by apply head_prim_reducible|].
       iIntros (X Hstep). apply head_reducible_prim_step in Hstep;[|done].
@@ -598,7 +625,7 @@ Proof using.
       eapply link_head_step_call_ext_2_inv in Hstep as (pubσ&privσ2&k2&->&?&?); eauto.
 
       iDestruct "Hcall" as (Ξ) "[HTΞ HΞ]".
-      iMod (@state_interp_split _ _ _ _ Λ2 with "Hσ2") as "[Hpub Hpriv2]"; first done.
+      iMod (state_interp_split with "Hσ2") as "[Hpub Hpriv2]"; first done.
       iMod (link_state_update _ Boundary with "Hob Hb") as "[Hob Hb]".
       do 3 iModIntro. iExists _, _. iSplitR; first done. simpl.
       iFrame "Hob Hpub Hpriv1 Hpriv2".
@@ -611,21 +638,21 @@ Proof using.
         assert (prog pe !! f = Some (inl fn1)) as Hpef.
         { rewrite lookup_union_l lookup_fmap. by rewrite Hf1. by rewrite Hf. }
 
-        (* administrative step CallS: LinkExprCall ~> LinkRunFunction *)
+        (* administrative step CallS: Link.ExprCall ~> LinkRunFunction *)
         iApply wp_link_call; first done.
-        (* administrative step RunFunction1S: LinkRunFunction ~> LinkExpr1 *)
+        (* administrative step RunFunction1S: LinkRunFunction ~> Link.Expr1 *)
         iApply (wp_link_run_function_1 with "Hb Hb1 HTΞ"); first done.
         iIntros (e1 He1) "Hwpcall Hb".
 
-        progress change (LkE (LinkExpr1 Λ1 Λ2 e1) [inr k2]) with
-          (linking.fill _ _ ([inr k2]:ectx (link_lang Λ1 Λ2)) (LkSE (LinkExpr1 Λ1 Λ2 e1))).
-        iApply (@wp_bind _ _ _ _ _ (link_lang Λ1 Λ2)).
-        iApply ((@wp_wand _ _ _ _ _ (link_lang Λ1 Λ2)) with "[Hwpcall Hb Hb2]").
+        progress change (Link.LkE (Link.Expr1 Λ1 Λ2 e1) [inr k2]) with
+          (Link.fill _ _ ([inr k2]:ectx (link_lang Λ1 Λ2)) (LkSE (Link.Expr1 Λ1 Λ2 e1))).
+        iApply wp_bind.
+        iApply (wp_wand with "[Hwpcall Hb Hb2]").
         { iDestruct "IH" as "#[IH1 _]". iApply ("IH1" with "Hwpcall [$Hb $Hb2]"). }
         iIntros (r) "[Hr (Hb & Hb1 & Hb2)]". iSpecialize ("HΞ" $! r).
         rewrite -fill_comp fill_empty. simpl.
 
-        (* administrative step Ret2S: LinkExprV ~> LinkExpr2 *)
+        (* administrative step Ret2S: Link.ExprV ~> Link.Expr2 *)
         iApply (wp_link_retval_2 with "[-Hb] Hb"). iIntros "Hb".
         (* continue the execution by induction *)
         iDestruct "IH" as "#[_ IH2]". iApply ("IH2" with "[-Hb Hb1] [$Hb $Hb1]"). unfold of_val.
@@ -634,29 +661,29 @@ Proof using.
       { (* external call *)
         iApply (wp_link_extcall_2 with "HTΞ HΞ [] [$Hb $Hb1 $Hb2]"); auto. iNext.
         iIntros (r) "HΞ Hb Hb1".
-        (* administrative step Ret1S: LinkExprV ~> LinkExpr1 *)
+        (* administrative step Ret1S: Link.ExprV ~> Link.Expr1 *)
         iApply (wp_link_retval_2 with "[-Hb] Hb"). iIntros "Hb".
         (* continue the execution by induction *)
         iDestruct "IH" as "#[_ IH2]". iApply ("IH2" with "HΞ [$Hb $Hb1]"). } }
 
     { (* WP: step case *)
       iDestruct "Hwp" as (Hred) "Hwp". iModIntro. iRight; iRight.
-      assert (head_reducible (prog pe) (LkSE (LinkExpr2 Λ1 Λ2 e2)) (LinkSt2 privσ1 σ2)).
+      assert (head_reducible (prog pe) (LkSE (Link.Expr2 Λ1 Λ2 e2)) (Link.St2 privσ1 σ2)).
       { destruct Hred as (? & Hstep).
-        exists (λ _, True). eapply Step2S. rewrite proj2_prog_union; [| apply Hcan_link].
+        exists (λ _, True). eapply Link.Step2S. rewrite proj2_prog_union; [| apply Hcan_link].
         all: eauto. }
       iSplitR; [by iPureIntro; apply head_prim_reducible|].
       iIntros (X Hstep). apply head_reducible_prim_step in Hstep;[|done].
       inversion Hstep; simplify_eq.
       { (* non-vacuous case: step in Λ2 *)
-        clear Hstep. rename H5 into Hstep.
+        clear Hstep. rename H4 into Hstep.
         rewrite proj2_prog_union in Hstep; [|apply Hcan_link].
         iSpecialize ("Hwp" $! _ Hstep). iMod "Hwp". iIntros "!>!>". iMod "Hwp" as (e' σ' HX) "[Hσ Hwp]".
         iModIntro. iExists _, _. iSplitR; [iPureIntro; naive_solver|]. iFrame "Hob Hσ Hpriv1".
         iDestruct "IH" as "[_ IH2]". iApply ("IH2" with "Hwp [$Hb $Hb1]"). }
       { exfalso. apply reducible_not_val in Hred. congruence. }
       { exfalso. clear Hstep. erewrite <-(of_to_class e0) in Hred; [|eassumption].
-        rewrite proj2_prog_union in H5;[|apply Hcan_link].
+        rewrite proj2_prog_union in H4;[|apply Hcan_link].
         destruct Hred as (?&Hred). eapply extcall_ctx_irreducible; eauto. } } }
 Qed.
 
